src/Step.v
@@ -1,12 +1,60 @@
-From Coq Require Import Lists.List.
+From Coq Require Import Logic.ChoiceFacts.
+From Coq Require Import Logic.Decidable.
 
 From STM Require Import Stm.
 
-(* Forward step definition *)
+(* State machine step definition *)
+Inductive Step S E (tr : Trans S E) (stm : Stm tr) : S -> S -> Prop :=
+| step (s1 : S) (e : E) (s2 : S) (tprf : tr s1 e s2)
+  : Step S E tr stm s1 s2.
 
-Inductive Step S E (stm : Stm S E) : S -> S -> Prop :=
-  | step (s1 : S) (e : E) (s2 : S)
-      (sprf : In (e, s2) (stm s1)) : Step S E stm s1 s2.
+Arguments Step {S} {E} _ {stm}.
+Arguments step {S} {E} _ {stm}.
 
-Arguments Step {S} {E}.
-Arguments step {S} {E}.
+(* State machine step theorems *)
+Theorem step_eq_etransstep : forall {S} {E} tr {stm : Stm tr} (s1 : S) (s2 : S),
+    (exists e : E, tr s1 e s2) <-> Step tr s1 s2.
+Proof.
+  intros S E tr stm s1 s2.
+  split.
+  - intros [e H].
+    apply (step tr s1 e s2).
+    apply H.
+  - intros H.
+    inversion H.
+    exists e.
+    apply tprf.
+Qed.
+
+Section Example.
+
+  Definition sem_step_decidable (s1 : Sem) (s2 : Sem) :
+      decidable (Step SemTrans s1 s2).
+    unfold decidable.
+    destruct s1.
+    - destruct s2.
+      + left. apply (step SemTrans _ Stop). constructor.
+      + left. apply (step SemTrans _ Next). constructor.
+      + right. intros H. inversion H. inversion tprf.
+      + left. apply (step SemTrans _ Fail). constructor.
+    - destruct s2.
+      + right. intros H. inversion H. inversion tprf.
+      + right. intros H. inversion H. inversion tprf.
+      + left. apply (step SemTrans _ Next). constructor.
+      + left. apply (step SemTrans _ Fail). constructor.
+    - destruct s2.
+      + left. apply (step SemTrans _ Next). constructor.
+      + right. intros H. inversion H. inversion tprf.
+      + left. apply (step SemTrans _ Stop). constructor.
+      + left. apply (step SemTrans _ Fail). constructor.
+    - right. intros H. inversion H. inversion tprf.
+  Defined.
+
+  Compute sem_step_decidable Green Black.
+
+  Example step_ex_1 : Step SemTrans Green Yellow.
+  Proof. apply (step SemTrans Green Next). constructor. Qed.
+
+  Check step SemTrans Green Next Yellow green_next.
+
+End Example.
