src/Stm.v
@@ -1,4 +1,65 @@
+From Coq Require Import Logic.Decidable.
+From Coq Require Import Program.Equality.
 
-(* State machine definition *)
+(* Transion *)
+Definition Trans S E := S -> E -> S -> Prop.
 
-Definition Stm S E := S -> list (E * S).
+(* State machine class *)
+Class Stm {S} {E} (trans : Trans S E) :=
+  { trans_funct (s1 : S) (e : E) (s2 : S) (s2' : S)
+    : trans s1 e s2 -> trans s1 e s2' -> s2 = s2' }.
+
+(* Decidable state machine class *)
+Class DecStm {S} {E} (trans : Trans S E) `{Stm S E trans} :=
+  { dec_trans (s1 : S) (e : E) (s2 : S) : decidable (trans s1 e s2) }.
+
+(* Functional transition tactic *)
+Ltac functional_transition :=
+    intros s1 e s2 s2' H1 H2;
+    dependent destruction H1;
+    repeat (dependent destruction H2; reflexivity).
+
+(* Decide transition tactic *)
+Ltac decide_transition s1 e s2:=
+  unfold decidable;
+  destruct s1, e, s2;
+  repeat ((left; constructor) + (right; intros H; inversion H)).
+
+Section Example.
+
+  Inductive Sem : Set :=
+  | Green
+  | Yellow
+  | Red
+  | Black.
+
+  Inductive Ev : Set :=
+  | Stop
+  | Next
+  | Fail.
+
+  Inductive SemTrans : Trans Sem Ev :=
+  | green_stop : SemTrans Green Stop Green
+  | green_next : SemTrans Green Next Yellow
+  | green_fail : SemTrans Green Fail Black
+  | yellow_next : SemTrans Yellow Next Red
+  | yellow_fail : SemTrans Yellow Fail Black
+  | red_stop : SemTrans Red Stop Red
+  | red_next : SemTrans Red Next Green
+  | red_fail : SemTrans Red Fail Black.
+
+  Theorem SemTrans_funct : forall (s1 : Sem) (e : Ev) (s2 : Sem) (s2' : Sem),
+      SemTrans s1 e s2 -> SemTrans s1 e s2' -> s2 = s2'.
+  Proof. functional_transition. Qed.
+
+  #[export] Instance SemTrans_Stm_inst : Stm SemTrans :=
+    { trans_funct := SemTrans_funct }.
+
+  Definition SemTrans_dec (s1 : Sem) (e : Ev) (s2 : Sem) :
+    decidable (SemTrans s1 e s2).
+  decide_transition s1 e s2. Defined.
+
+  #[export] Instance SemTrans_DecStm_inst : DecStm SemTrans :=
+    { dec_trans := SemTrans_dec }.
+
+End Example.
